LynxTest.lean
@@ -7,6 +7,7 @@ import LynxTest.Term.Map
 import LynxTest.Tactic.Contracts
 import LynxTest.Tactic.Recursive
 import LynxTest.Tactic.Opaque
+import LynxTest.Tactic.Pure
 import LynxTest.Tactic.Failures
 import LynxTest.Modules.Extensions
 import LynxTest.Modules.Erlang
